LeanFixpoint/Solve/Weaken.lean
@@ -108,9 +108,6 @@ partial def weakenOnce
       -- specialize clause with that κ and current solutions
       -- note: below performs κ specialization for all the clauses
       let vc ← (specializeClauseForHead headKVar q slots currentSols fc).run kctx
-      let vcFmt ← ppExpr vc
-      let qFmt ← ppExpr q
-      IO.println s!"[weakenOnce] head={headKVar.name} slots={slots} q={qFmt} vc={vcFmt}"
       if ← checkExprVC vc then
         IO.println s!"[weakenOnce] KEEPING IT"
         kept := kept.concat (q, slots)
